add leaps and forward analysis

deps/poulet4/lib/P4automata/BisimChecker.v
@@ -4,6 +4,9 @@ Require Import Poulet4.P4automata.P4automaton.
 Require Import Poulet4.P4automata.PreBisimulationSyntax.
 Require Poulet4.P4automata.WP.
 Require Poulet4.P4automata.WPSymBit.
+Require Poulet4.P4automata.WPSymLeap.
+Require Poulet4.P4automata.Reachability.
+
 Import List.ListNotations.
 
 Section BisimChecker.
@@ -26,7 +29,6 @@ Section BisimChecker.
 
   Variable (a: P4A.t S H).
 
-  Check WP.wp.
   Variable (wp: P4A.t S H ->
                 conf_rel S H ->
                 list (conf_rel S H)).
@@ -86,14 +88,18 @@ Arguments pre_bisimulation {S1 S2 H equiv2 H_eq_dec} a wp.
 Require Import Poulet4.P4automata.Examples.
 
 Notation init_conf := (inl Simple.Start, [], []).
-Notation "⟨ s1 , n1 ⟩ ⟨ s2 , n2 ⟩ ⊢ b" :=
+
+Notation "ctx , ⟨ s1 , n1 ⟩ ⟨ s2 , n2 ⟩ ⊢ b" :=
   ({| cr_st :=
         {| cs_st1 := {| st_state := s1; st_buf_len := n1 |};
            cs_st2 := {| st_state := s2; st_buf_len := n2 |}; |};
+      cr_ctx := ctx;
       cr_rel := b|}) (at level 10).
+Notation btrue := (BRTrue _ _).
+Notation bfalse := (BRFalse _ _).
+Notation "a ⇒ b" := (BRImpl a b) (at level 40).
 
-
-Section SumInitRel.
+Section InitRels.
   Set Implicit Arguments.
   Variables (S1 S2 H: Type).
   Context `{S1_fin: Finite S1}.
@@ -115,8 +121,34 @@ Section SumInitRel.
 
   Definition sum_init_rel (a: P4A.t (S1 + S2) H) : crel (S1 + S2) H := 
     List.concat (List.map (sum_not_accept1 a) (enum S1)
-                 ++ List.map (sum_not_accept2 a) (enum S2)).
-End SumInitRel.
+                          ++ List.map (sum_not_accept2 a) (enum S2)).
+
+  Definition reachable_pair_to_partition '((s1, s2): Reachability.state_pair _ _)
+    : crel (S1 + S2) H :=
+    match s1.(st_state) with
+    | inl st =>
+      [BCEmp, ⟨inl st, s1.(st_buf_len)⟩ ⟨inr true, 0⟩ ⊢ bfalse]
+    | inr st =>
+      []
+    end
+      ++
+      match s2.(st_state) with
+      | inl st =>
+        [BCEmp, ⟨inr true, 0⟩ ⟨inl st, s2.(st_buf_len)⟩ ⊢ bfalse]
+      | inr st =>
+        []
+      end.
+
+  Definition reachable_pairs_to_partition (r: Reachability.state_pairs _ _)
+    : crel (S1 + S2) H :=
+    List.concat (List.map reachable_pair_to_partition r).
+
+  Definition mk_init (n: nat) (a: P4A.t (S1 + S2) H) s1 s2 :=
+    let s := ({| st_state := inl (inl s1); st_buf_len := 0 |}, 
+              {| st_state := inl (inr s2); st_buf_len := 0 |}) in
+    reachable_pairs_to_partition
+      (Reachability.reachable_states a 1000 [s]).
+End InitRels.
 
 Ltac pbskip :=
   apply PreBisimulationSkip;
@@ -155,17 +187,24 @@ Ltac pbskip' :=
 
 Ltac solve_bisim' :=
   match goal with
+  | |- context[WPSymLeap.wp _ _] =>
+    progress (
+        unfold WPSymLeap.wp at -1;
+        autounfold with wp;
+        unfold WP.wp_op;
+        simpl)
   | |- context[WPSymBit.wp _ _] =>
     progress (
         unfold WPSymBit.wp at -1;
         unfold
-                WP.wp, WP.wp_pred_pair, WP.st_pred, WP.wp_pred, WP.wp_op,
+                WP.preds, WP.wp_pred_pair, WP.st_pred, WP.wp_pred, WP.wp_op,
                 WPSymBit.wp_pred_pair 
               ; simpl)
   | |- context[WP.wp _ _] =>
-    progress (unfold
-                WP.wp, WP.wp_pred_pair, WP.st_pred, WP.wp_pred, WP.wp_op,
-                WPSymBit.wp, WPSymBit.wp_pred_pair 
+    progress (
+        unfold WP.wp at -1;
+        unfold
+                WP.preds, WP.wp_pred_pair, WP.st_pred, WP.wp_pred, WP.wp_op
               ; simpl)
   | |- pre_bisimulation _ _ _ [] _ _ => apply PreBisimulationClose
   | |- pre_bisimulation _ _ _ (_::_) _ _ => pbskip'
@@ -173,10 +212,7 @@ Ltac solve_bisim' :=
   | |- _ => progress simpl
   end.
 
-Notation btrue := (BRTrue _ _).
-Notation bfalse := (BRFalse _ _).
-Notation "a ⇒ b" := (BRImpl a b) (at level 40).
-
+(*
 Lemma prebisim_simple_split:
   pre_bisimulation SimpleSplit.aut
                    (WP.wp (H:=SimpleSplit.header))
@@ -186,9 +222,6 @@ Lemma prebisim_simple_split:
                    (inl (inr Split.StSplit1), [], []).
 Proof.
   unfold sum_init_rel.
-  simpl.
-  apply PreBisimulationExtend.
-  simpl.
   time (repeat solve_bisim').
   cbv in *.
   intuition (try congruence).
@@ -203,11 +236,114 @@ Lemma prebisim_simple_split_sym:
                    (inl (inr Split.StSplit1), [], []).
 Proof.
   unfold sum_init_rel.
-  simpl.
-  apply PreBisimulationExtend.
-  simpl.
+  do 90 solve_bisim'.
+  do   5 solve_bisim'.
+  do   5 solve_bisim'.
+  do   5 solve_bisim'.
+  do   5 solve_bisim'.
+  do   5 solve_bisim'.
+  do   5 solve_bisim'.
+  do   5 solve_bisim'.
+  do   5 solve_bisim'.
+  do   5 solve_bisim'.
+  do   5 solve_bisim'.
+  do   5 solve_bisim'.
+  do   5 solve_bisim'.
+  do   5 solve_bisim'.
+  do   5 solve_bisim'.
+  do   5 solve_bisim'.
+  do   5 solve_bisim'.
+  do   5 solve_bisim'.
+  do 40 solve_bisim'.
+  do 40 solve_bisim'.
+  do 40 solve_bisim'.
+  do 40 solve_bisim'.
+  do 40 solve_bisim'.
+  do 40 solve_bisim'.
+  do 40 solve_bisim'.
+  do 40 solve_bisim'.
+  do 40 solve_bisim'.
+  do 40 solve_bisim'.
+  do 40 solve_bisim'.
+  do 32 solve_bisim'.
+  do 32 solve_bisim'.
+  do 32 solve_bisim'.
+  do 32 solve_bisim'.
+  do 32 solve_bisim'.
+  time (repeat (time solve_bisim')).
+  cbv in *.
+  intuition (try congruence).
+Qed.
+
+Lemma prebisim_simple_split_sym_leap:
+  pre_bisimulation SimpleSplit.aut
+                   (WPSymLeap.wp (H:=SimpleSplit.header))
+                   nil
+                   (sum_init_rel SimpleSplit.aut)
+                   (inl (inl Simple.Start), [], [])
+                   (inl (inr Split.StSplit1), [], []).
+Proof.
+  unfold sum_init_rel.
+  do 200 solve_bisim'.
+  cbv in *.
+  intuition (try congruence).
+Qed.
+*)
+
+Definition possibly_unsound_init_rel
+  : crel (Simple.state + Split.state) (Sum.H Simple.header Split.header)
+  :=
+    [BCEmp, ⟨inl (inl Simple.Start), 0⟩ ⟨inr true, 0⟩ ⊢ bfalse;
+    BCEmp, ⟨inl (inl Simple.Start), 4⟩ ⟨inr true, 0⟩ ⊢ bfalse;
+    BCEmp, ⟨inr true, 0⟩ ⟨inl (inr Split.StSplit1), 0⟩ ⊢ bfalse;
+    BCEmp, ⟨inr true, 0⟩ ⟨inl (inr Split.StSplit2), 0⟩ ⊢ bfalse].
+
+
+Definition possibly_unsound_init_rel'
+  : crel (Simple.state + Split.state) (Sum.H Simple.header Split.header)
+  :=
+    Eval compute in (mk_init 10 SimpleSplit.aut Simple.Start Split.StSplit1). 
+
+(*
+Lemma prebisim_simple_split_small_init:
+  pre_bisimulation SimpleSplit.aut
+                   (WP.wp (H:=SimpleSplit.header))
+                   nil
+                   (sum_init_rel SimpleSplit.aut)
+                   (inl (inl Simple.Start), [], [])
+                   (inl (inr Split.StSplit1), [], []).
+Proof.
+  unfold sum_init_rel.
+  time (repeat solve_bisim').
+  cbv in *.
+  intuition (try congruence).
+Qed.
+*)
+
+Lemma prebisim_simple_split_sym_small_init:
+  pre_bisimulation SimpleSplit.aut
+                   (WPSymBit.wp (H:=SimpleSplit.header))
+                   nil
+                   possibly_unsound_init_rel'
+                   (inl (inl Simple.Start), [], [])
+                   (inl (inr Split.StSplit1), [], []).
+Proof.
+  unfold possibly_unsound_init_rel'.
   time (repeat solve_bisim').
   cbv in *.
   intuition (try congruence).
 Qed.
 
+Lemma prebisim_simple_split_sym_leap_small_init:
+  pre_bisimulation SimpleSplit.aut
+                   (WPSymLeap.wp (H:=SimpleSplit.header))
+                   nil
+                   possibly_unsound_init_rel'
+                   (inl (inl Simple.Start), [], [])
+                   (inl (inr Split.StSplit1), [], []).
+Proof.
+  unfold possibly_unsound_init_rel'.
+  time (repeat solve_bisim').
+  cbv in *.
+  intuition (try congruence).
+Qed.
