deps/poulet4/lib/P4automata/Reachability.v
@@ -1,0 +1,98 @@
+Require Import Coq.Classes.EquivDec.
+Require Import Coq.Relations.Relations.
+Require Import Coq.Program.Program.
+Require Import Poulet4.FinType.
+Require Import Poulet4.P4automata.P4automaton.
+Require Import Poulet4.P4automata.PreBisimulationSyntax.
+Require Poulet4.P4automata.WP.
+Require Poulet4.P4automata.WPSymBit.
+Require Poulet4.P4automata.WPSymLeap.
+
+Import List.ListNotations.
+
+Set Implicit Arguments.
+Section ReachablePairs.
+
+  (* State identifiers. *)
+  Variable (S1: Type).
+  Context `{S1_eq_dec: EquivDec.EqDec S1 eq}.
+  Context `{S1_finite: @Finite S1 _ S1_eq_dec}.
+
+  Variable (S2: Type).
+  Context `{S2_eq_dec: EquivDec.EqDec S2 eq}.
+  Context `{S2_finite: @Finite S2 _ S2_eq_dec}.
+
+  Definition S: Type := S1 + S2.
+
+  (* Header identifiers. *)
+  Variable (H: Type).
+  Context `{H_eq_dec: EquivDec.EqDec H eq}.
+  Context `{H_finite: @Finite H _ H_eq_dec}.
+
+  Variable (a: P4A.t S H).
+
+  Notation conf := (configuration (P4A.interp a)).
+
+  Definition state_pair : Type :=
+    state_template S * state_template S.
+  Global Program Instance state_pair_eq_dec: EquivDec.EqDec state_pair eq :=
+    { equiv_dec x y :=
+        if Sumbool.sumbool_and _ _ _ _
+             (state_template_eq_dec (fst x) (fst y))
+             (state_template_eq_dec (snd x) (snd y))
+        then in_left
+        else in_right }.
+  Next Obligation.
+    destruct x, y.
+    simpl in *.
+    congruence.
+  Qed.
+  Next Obligation.
+    intuition.
+  Qed.
+
+  Definition state_pairs : Type :=
+    list state_pair.
+
+  Definition possible_next_states (st: P4A.state S H) : list (P4A.state_ref S) :=
+    match st.(P4A.st_trans) with
+    | P4A.TGoto _ s' =>
+      [s']
+    | P4A.TSel _ cases default =>
+      default :: List.map (fun c => P4A.sc_st c) cases
+    end.
+
+  Definition reads_left (s: S) (buf_len: nat) :=
+    P4A.size a s - buf_len.
+
+  Definition advance (steps: nat) (t1: state_template S) (st: P4A.state S H) :=
+    if t1.(st_buf_len) + steps == P4A.state_size st
+    then List.map (fun r => {| st_state := r; st_buf_len := 0 |}) (possible_next_states st)
+    else [{| st_state := t1.(st_state); st_buf_len := t1.(st_buf_len) + steps |}].
+
+  Definition reachable_pair_step (r0: state_pair) : state_pairs :=
+    let '(t1, t2) := r0 in
+    match t1.(st_state), t2.(st_state) with
+    | inl s1, inl s2 => 
+      let st1 := P4A.t_states a s1 in
+      let st2 := P4A.t_states a s2 in
+      let len1 := t1.(st_buf_len) in
+      let len2 := t2.(st_buf_len) in
+      let steps := Nat.min (reads_left s1 len1)
+                           (reads_left s2 len2) in
+      List.list_prod (advance steps t1 st1)
+                     (advance steps t2 st2)
+    | _, _ => [] (* is this right? *)
+    end.
+  
+  Definition reachable_step (r: state_pairs) : state_pairs :=
+    let r' := (List.concat (List.map reachable_pair_step r)) in
+    List.nodup state_pair_eq_dec (r' ++ r).
+
+  Fixpoint reachable_states (fuel: nat) (r: state_pairs) :=
+    match fuel with
+    | 0 => r
+    | Datatypes.S fuel => reachable_states fuel (reachable_step r)
+    end.
+
+End ReachablePairs.
